edit examples

verified/mutation.dfy
@@ -105,10 +105,10 @@ module MutationModule {
   }
 
   function EnsureImmVector(o: vec, m: vec, imm: immutables): vec
-    ensures var m' := EnsureImmVector(o, m, imm);
-            (forall i: idx :: m'[i] == if i in imm then o[i] else m[i]) &&
-            ImmutableVecCorrect(o, m', imm)  &&
-            (ImmutableVecCorrect(o, m, imm) ==> m == m')
+    ensures ImmutableVecCorrect(o, EnsureImmVector(o, m, imm), imm)
+    ensures ImmutableVecCorrect(o, m, imm) ==> m == EnsureImmVector(o, m, imm)
+    ensures forall i :: i in imm ==> EnsureImmVector(o, m, imm)[i] == o[i]
+    ensures forall i: idx :: i !in imm ==> EnsureImmVector(o, m, imm)[i]==m[i]
   {
     MapVec(o, m, IRow(imm))
   }
@@ -189,6 +189,7 @@ module MutationModule {
     else [VectMutation(o[0], m[0], mut, imm)] +
          ControlledMutation(o[1..], m[1..], mut, imm)
   }
+
 }
 
 // To configure value type and dimensionality
@@ -208,13 +209,15 @@ module Tests {
   type domain = V.D
 
   // for some reason |s| > 1 is easier than |s| == 2
-  predicate P(s: seq<domain>) {
+  predicate P(s: seq<domain>)
+  {
     |s| > 1 && s[0] <= s[1]
   }
 
   // Invariants
   const imm := [0, 3, 4]
   const mut := [([1, 3], P)]
+  const I := mut[0]
 
   const RealSample := (
     [[-2.3, 1.8, 5.0, 4.1, 7.2], [82.2, 1.3, 7.6, 4.8, 6.3]],
@@ -223,56 +226,78 @@ module Tests {
     [[-2.3, 3.2, 5.5, 4.1, 7.2], [82.2, 1.3, 7.6, 4.8, 6.3]])
 
   const IntSample := (
-    [[-2, 1, 4, 7, -3], [11, 2, -7, 5, 3]],
-    [[-3, 2, 5, 8, -4], [10, 6, -5, 4, 2]],
-    [[-2, 2, 5, 7, -3], [11, 6, -5, 5, 3]],
-    [[-2, 2, 5, 7, -3], [11, 2, -7, 5, 3]])
+    [[-2, 1, 4, 7, -3], [11, 2, -7, 5, 3]], // [X] initial
+    [[-3, 2, 5, 8, -4], [10, 6, -5, 4, 2]], // [Y] mutation
+    [[-2, 2, 5, 7, -3], [11, 6, -5, 5, 3]], // mid-[T]ransform
+    [[-2, 2, 5, 7, -3], [11, 2, -7, 5, 3]]) // [E]xpected (final)
 
   const source := IntSample
-  const X := source.0
-  const Y := source.1
-  const T := source.2
-  const E := source.3 // expected
+  const X := source.0 // [X] initial
+  const Y := source.1 // [Y] mutation
+  const T := source.2 // mid-[T]ransform
+  const E := source.3 // [E]xpected (final)
 
-  method Basics()
+  method CheckPremises()
+    ensures V.MutableHold(X, mut)
+    ensures !V.MutableHold(Y, mut)
   {
+    // initial input is satisfactory
     assert V.MutableHold(X, mut);
 
+    // the mutation does not preserve all invariants
     assert (V.MutableHold(Y, mut) == false) by {
       assert V.MutableVecCorrect(Y[1], mut) == false;
     }
   }
 
-  method ImmutableTransfrom()
+  method EnsureImmRestoresImmutableIndices()
+    ensures forall i : nat :: i < |X| ==>
+      var vi := V.EnsureImmVector(X[i], Y[i], imm);
+      V.ImmutableVecCorrect(X[i], vi, imm)
   {
     var T0 := V.EnsureImmVector(X[0], Y[0], imm);
-    var T1 := V.EnsureImmVector(X[1], Y[1], imm);
-    assert T0 == T[0] && T1 == T[1];
-
     assert V.ImmutableVecCorrect(X[0], T0, imm);
-    assert V.ImmutableVecCorrect(X[1], T1, imm);
 
-    assert V.EvalPred(T0, mut[0]) == true;
-    assert V.EvalPred(T1, mut[0]) == false;
+    var T1 := V.EnsureImmVector(X[1], Y[1], imm);
+    assert V.ImmutableVecCorrect(X[1], T1, imm);
+  }
+
+  method MutableTransfrom()
+    ensures V.MutableVecCorrect(V.EnsureImmVector(X[0], Y[0], imm), mut)
+    ensures !V.MutableVecCorrect(V.EnsureImmVector(X[1], Y[1], imm), mut)
+  {
+    // Mutation predicates hold for T0
+    assert V.EvalPred(X[0], I);
+    var T0 := V.EnsureImmVector(X[0], Y[0], imm);
+    assert V.EvalPred(T0, I);
+
+    // Mutation predicates fail for T1
+    assert V.EvalPred(X[1], I);
+    var T1 := V.EnsureImmVector(X[1], Y[1], imm);
+    assert V.EvalPred(T1, mut[0]) == false by {
+      assert T1[1] == Y[1][1];
+      assert T1[3] == X[1][3];
+      assert !(T1[1] <= T1[3]);
+    }
   }
 
   method Main() {
+
+    CheckPremises();
+    EnsureImmRestoresImmutableIndices();
+    MutableTransfrom();
 
     var Y' := V.ControlledMutation(X, Y, mut, imm);
     assert V.IsCorrect(X, Y', mut, imm);
 
     var T0 := V.EnsureImmVector(X[0], Y[0], imm);
-    assert V.MutableVecCorrect(T0, mut);
-    assert Y'[0]
-        == V.VectMutation(X[0], Y[0], mut, imm)
-        == V.EnsureMutVector(X[0], T0, mut)
-        == E[0] == T0;
+    assert T0 == V.EnsureMutVector(X[0], T0, mut) == Y'[0];
 
     var T1 := V.EnsureImmVector(X[1], Y[1], imm);
-    assert V.MutableVecCorrect(T1, mut) == false;
-    assert Y'[1]
-        == V.VectMutation(X[1], Y[1], mut, imm)
-        == V.EnsureMutVector(X[1], T1, mut)
-        == E[1] == X[1];
+    assert !V.MutableVecCorrect(T1, mut);
+    assert X[1] 
+            == V.EnsureMutVector(X[1], T1, mut)
+            == V.VectMutation(X[1], Y[1], mut, imm) 
+            == Y'[1];
   }
 }
